
<handout xml:id="handout-section-2-1-matrix-algebra">
  <title>2.1 Matrix Operations</title>

  <page xml:id="p-2-1-overview">
    <title>Topics and Objectives</title>

    <objectives>
        <title>Topics</title>
    <ul>
      <li>Identity and zero matrices</li>
      <li>Matrix algebra (sums and products, scalar multiplies, matrix powers)</li>
      <li>Transpose of a matrix</li>
    </ul>
    </objectives>

    <objectives workspace="true">
        <title>Goals</title>
    <ul>
      <li>
        <em>Apply</em> matrix algebra, the matrix transpose, and the zero and identity matrices,
        to <em>solve</em> and <em>analyze</em> matrix equations.
      </li>
    </ul>
    </objectives>

    <p><nbsp/></p>

    <definition xml:id="def-zero-matrix" workspace="true">
      <title>Zero Matrix</title>
      <statement>
        <p>
          A <term>zero matrix</term> is any matrix whose every entry is zero.
        </p>
        <me>
          0_{2\times 3}=
          \begin{bmatrix}
            0 \amp 0 \amp 0\\
            0 \amp 0 \amp 0
          \end{bmatrix},
          \qquad
          0_{2\times 1}=
          \begin{bmatrix}
            0\\
            0
          \end{bmatrix}.
        </me>
      </statement>
    </definition>


    <definition xml:id="def-identity-matrix" workspace="true">
      <title>Identity Matrix</title>
      <statement>
        <p>
          The <m>n\times n</m> <term>identity matrix</term> has ones on the main diagonal and zeros elsewhere.
        </p>
        <me>
          I_2=
          \begin{bmatrix}
            1 \amp 0\\
            0 \amp 1
          \end{bmatrix},
          \qquad
          I_3=
          \begin{bmatrix}
            1 \amp 0 \amp 0\\
            0 \amp 1 \amp 0\\
            0 \amp 0 \amp 1
          \end{bmatrix}.
        </me>
      </statement>
    </definition>

    <p><nbsp/></p>

    <p>
      Note: Any matrix with dimensions <m>n\times n</m> is <term>square</term>.
      Zero matrices need not be square; identity matrices must be square.
    </p>

    <p><nbsp/></p>
  </page>


  <page xml:id="p-2-1-sums-scalars">
    <title>Sums and Scalar Multiples</title>

    <p>
      Suppose <m>A\in\mathbb{R}^{m\times n}</m>, and <m>a_{i,j}</m> is the element of <m>A</m>
      in row <m>i</m> and column <m>j</m>.
    </p>

    <ol>
      <li>
        <p>
          If <m>A</m> and <m>B</m> are <m>m\times n</m> matrices, then the elements of <m>A+B</m>
          are <m>a_{i,j}+b_{i,j}</m>.
        </p>
      </li>
      <li>
        <p>
          If <m>c\in\mathbb{R}</m>, then the elements of <m>cA</m> are <m>c\,a_{i,j}</m>.
        </p>
      </li>
    </ol>

    <example xml:id="ex-sum-scalar-find-c-k" workspace="true">
      <statement>
        <p>
          If
        </p>
        <me>
          \begin{bmatrix}
            1 \amp 2 \amp 3\\
            4 \amp 5 \amp 6
          \end{bmatrix}
          + c
          \begin{bmatrix}
            7 \amp 4 \amp 7\\
            0 \amp 0 \amp k
          \end{bmatrix}
          =
          \begin{bmatrix}
            15 \amp 10 \amp 17\\
            4 \amp 5 \amp 16
          \end{bmatrix},
        </me>
        <p>
          what are the values of <m>c</m> and <m>k</m>?
        </p>
      </statement>
      <solution>
        <p>
            Note that we can use rules (a) and (b) above to combine the left expression and get the following equation: <me>\begin{bmatrix} 1 + 7c \amp 2 + 4c \amp 3 + 7c \\ 4 \amp 5 \amp 6 + kc \end{bmatrix} = \begin{bmatrix} 15 \amp 10 \amp 17 \\ 4 \amp 5 \amp 16 \end{bmatrix}</me> Setting corresponding entries equal to one another, we see that <m>c = 2</m> and <m>k = 5</m>.
        </p>
      </solution>
    </example>

    <p><nbsp/></p>
  </page>


  <page xml:id="p-2-1-properties-addition-scalars">
    <title>Properties of Sums and Scalar Multiples</title>

    <p>
      Scalar multiples and matrix addition have the expected properties.
      If <m>r,s\in\mathbb{R}</m> are scalars and <m>A,B,C</m> are <m>m\times n</m> matrices, then:
    </p>

    <ol>
      <li><m>A + 0_{m\times n} = A</m></li>
      <li><m>(A+B)+C = A+(B+C)</m></li>
      <li><m>r(A+B)=rA+rB</m></li>
      <li><m>(r+s)A = rA + sA</m></li>
      <li><m>r(sA) = (rs)A</m></li>
    </ol>

    <p><nbsp/></p>


    <definition xml:id="def-matrix-multiplication-columns" workspace="true">
      <title>Matrix Product via Columns</title>
      <statement>
        <p>
          Let <m>A</m> be an <m>m\times n</m> matrix and <m>B</m> be an <m>n\times p</m> matrix.
          The product <m>AB</m> is an <m>m\times p</m> matrix, given by
        </p>
        <me>
          AB
          =
          A
          \begin{bmatrix}
            \vec b_1 \amp \cdots \amp \vec b_p
          \end{bmatrix}
          =
          \begin{bmatrix}
            A\vec b_1 \amp \cdots \amp A\vec b_p
          \end{bmatrix}.
        </me>
      </statement>
    </definition>

    <p>
      Note: The dimensions of <m>A</m> and <m>B</m> determine whether <m>AB</m> is defined,
      and what its dimensions will be.
    </p>

    <image xml:id="img-matrix-multiplication-dimensions" source="./matrix_multi2.png" width="40%">
      <shortdescription>Diagram showing how matrix dimensions match in a product.</shortdescription>
      <description>
        A visual guide to when <m>AB</m> is defined based on inner dimensions.
      </description>
    </image>

    <p><nbsp/></p>
  </page>


  <page xml:id="p-2-1-row-column-rule">
    <title>Row-Column Rule</title>

    <theorem xml:id="thm-row-column-rule">
      <title>Row-Column Rule for Matrix Multiplication</title>
      <statement>
        <p>
          If <m>A\in\mathbb{R}^{m\times n}</m> has rows <m>\vec a_i</m> and
          <m>B\in\mathbb{R}^{n\times p}</m> has columns <m>\vec b_j</m>, then each element of
          <m>C=AB</m> is
        </p>
        <me>
          c_{ij}=\vec a_i\cdot \vec b_j.
        </me>
      </statement>
    </theorem>

    <p><nbsp/></p>

    <example xml:id="ex-row-column-compute" workspace="true">
      <statement>
        <p>Compute the following using the row-column method.</p>
        <me>
          C=AB=
          \begin{bmatrix}
            2 \amp 0\\
            1 \amp -1
          \end{bmatrix}
          \begin{bmatrix}
            3 \amp 0 \amp 1\\
            4 \amp 5 \amp 6
          \end{bmatrix}.
        </me>
      </statement>
      <solution>
        <p>
            Note that 
        </p>
            <m> \begin{eqnarray*} AB \amp = \amp \begin{bmatrix} 2 \amp 0 \\ 1 \amp -1 \end{bmatrix}\begin{bmatrix} 3 \amp 0 \amp 1 \\ 4 \amp 5 \amp 6 \end{bmatrix}\\ \amp = \amp \begin{bmatrix} 2 \cdot 3 + 0 \cdot 4 \amp 2 \cdot 0 + 0 \cdot 5 \amp 2 \cdot 1 + 0 \cdot 6 \\ 1 \cdot 3 + (-1) \cdot 4 \amp 1 \cdot 0 + (-1) \cdot 5 \amp 1 \cdot 1 + (-1) \cdot 6 \end{bmatrix}\\ \amp = \amp \begin{bmatrix} 6 \amp 0 \amp 2 \\ -1 \amp -5 \amp -5 \end{bmatrix}\end{eqnarray*}</m> 
            <p>Note that this method is faster than using the original definition of matrix multiplication given in <xref ref="def-matrix-multiplication-columns"/>. For example, to compute the first column of <m>AB </m> using the original definition, we would compute the following: <me>\begin{bmatrix}2 \amp 0 \\ 1 \amp -1 \end{bmatrix}\begin{bmatrix} 3 \\ 4 \end{bmatrix} = 3\begin{bmatrix} 2 \\ 1\end{bmatrix} + 4 \begin{bmatrix} 0 \\ -1 \end{bmatrix} = \begin{bmatrix} 6 \\ -1 \end{bmatrix}</me>
        </p>
      </solution>
    </example>

    <p><nbsp/></p>
  </page>


  <page xml:id="p-2-1-properties-multiplication">
    <title>Properties and Warnings</title>
    <theorem workspace="true" xml:id="thm-properties-multiplication">
        <title> Properties and Warnings</title>
            <p>
            Let <m>A,B,C</m> be matrices of sizes needed for the products to be defined,
            and suppose <m>A</m> is <m>m\times n</m>.
            </p>

            <ol>
            <li><p><em>Associative:</em> <m>(AB)C = A(BC)</m></p></li>
            <li><p><em>Left distributive:</em> <m>A(B+C)=AB+AC</m></p></li>
            <li><p><em>Right distributive:</em> <m>(A+B)C = AC + BC</m></p></li>
            <li><p><em>Identity:</em> <m>I_m A = A I_n</m></p></li>
            </ol>

            <p><em>Warnings:</em></p>
            <ol>
            <li>
                <p><em>Non-commutative:</em> In general, <m>AB\neq BA</m>.</p>
            </li>
            <li>
                <p><em>Non-cancellation:</em> <m>AB=AC</m> does not imply <m>B=C</m>.</p>
            </li>
            <li>
                <p><em>Zero divisors:</em> <m>AB=0</m> does not imply <m>A=0</m> or <m>B=0</m>.</p>
            </li>
            </ol>
        </theorem>

        <p><nbsp/></p>

    <p>
      The associative property is <m>(AB)C = A(BC)</m>. If <m>C=\vec x</m>, then:
    </p>

    <me>(AB)\vec x = A(B\vec x).</me>

    <p>Schematically:</p>

    <image xml:id="img-associative-flow" width="70%">
      <latex-image>
        <latex>
% TikZ styles (as in the TeX source)
\tikzstyle{startstop} =[trapezium, trapezium left angle=70, trapezium right angle=110,
  minimum width=1cm, minimum height=1cm, text centered, fill=red!30]
\tikzstyle{io} = [trapezium, trapezium left angle=70, trapezium right angle=110,
  minimum width=1cm, minimum height=1cm, text centered, fill=blue!30]
\tikzstyle{process} = [trapezium, trapezium left angle=70, trapezium right angle=110,
  minimum width=1cm, minimum height=1cm, text centered, fill=orange!30]
\tikzstyle{arrow} = [thick,->,>=stealth]

\begin{tikzpicture}[node distance=2cm]
  \node(x)  [startstop] {$\vec x$};
  \node(bx) [io, below of=x] {$B\vec x$};
  \node(abx)[process, right of=x,xshift=4cm]{$AB\vec x$};

  \draw [arrow] (x) -- node[anchor=east] {\small Multiplication by $B$} (bx);
  \draw [arrow] (bx) -- node[anchor=north,xshift=1cm] {\small Multiplication by $A$} (abx);
  \draw [arrow] (x) -- node[anchor=south] {\small Multiplication by $AB$} (abx);
\end{tikzpicture}
        </latex>
      </latex-image>
      <shortdescription>Flow diagram comparing two ways to multiply matrices.</shortdescription>
      <description>
        Diagram showing two ways of getting from <m>\vec x</m> to <m>AB\vec x</m>, either by  <m>\vec x \mapsto B\vec x \mapsto AB\vec x</m> or by direct multiplication by <m>\vec x \mapsto AB\vec x</m>.
      </description>
    </image>

    <p>
      The product <m>AB\vec x</m> can be obtained either by multiplying by <m>AB</m>,
      or by multiplying by <m>B</m> and then by <m>A</m>. This corresponds to
      <em>composition of linear transformations</em>.
    </p>

    <p><nbsp/></p>
  </page>



  <page xml:id="p-2-1-noncomm-example">
    <title>Example: Non-Commutativity</title>

    <example xml:id="ex-noncomm-with-A" workspace="true">
      <statement>
        <p>Let</p>
        <me>
          A=
          \begin{bmatrix}
            1 \amp 1\\
            0 \amp 0
          \end{bmatrix}.
        </me>
        <p>
          Give an example of a <m>2\times 2</m> matrix <m>B</m> such that <m>AB\neq BA</m>.
        </p>
      </statement>
      <solution>
        <p>
            Honestly, pretty much any matrix you choose at random will work. For example, let <m>B = \begin{bmatrix} 1 \amp 2 \\ 3 \amp 4 \end{bmatrix}</m> and note that <me>AB = \begin{bmatrix} 1 \amp 1 \\ 0 \amp 0 \end{bmatrix}\begin{bmatrix}1 \amp 2 \\ 3 \amp 4 \end{bmatrix} = \begin{bmatrix} 1 \cdot 1 + 1 \cdot 3 \amp 1 \cdot 2 + 1 \cdot 4 \\ 0 \cdot 1 + 0 \cdot 3 \amp 0 \cdot 2 + 0 \cdot 4 \end{bmatrix} = \begin{bmatrix} 4 \amp 6 \\ 0 \amp 0 \end{bmatrix}</me>, while <me>BA = \begin{bmatrix} 1 \amp 2 \\ 3 \amp 4 \end{bmatrix}\begin{bmatrix} 1 \amp 1 \\ 0 \amp 0 \end{bmatrix} = \begin{bmatrix} 1 \cdot 1 + 2 \cdot 0 \amp 1 \cdot 1 + 2 \cdot 0 \\ 3 \cdot 1 + 4 \cdot 0 \amp 3 \cdot 1 + 4 \cdot 0 \end{bmatrix} = \begin{bmatrix} 1 \amp 1 \\ 3 \amp 3 \end{bmatrix}</me>. Therefore, <m>AB \neq BA </m>.
        </p>
      </solution>
    </example>

    <p><nbsp/></p>
  </page>


  <page xml:id="p-2-1-transpose">
    <title>The Transpose of a Matrix</title>

    <definition xml:id="def-transpose">
      <title>Transpose</title>
      <statement>
        <p>
          The <term>transpose</term> <m>A^T</m> is the matrix whose columns are the rows of <m>A</m>.
        </p>
      </statement>
    </definition>

    <p><nbsp/></p>

    <example xml:id="ex-transpose-compute" workspace="true">
      <statement>
        <p>Compute:</p>
        <me>
          A = \begin{bmatrix}
            1 \amp 2 \amp 3 \amp 4 \amp 5\\
            0 \amp 1 \amp 0 \amp 2 \amp 0
          \end{bmatrix}^T
        </me>
      </statement>
      <solution>
        <p>
            We have that <m>A^T = \begin{bmatrix} 1 \amp 0 \\ 2 \amp 1 \\ 3 \amp 0 \\ 4 \amp 2 \\ 5 \amp 0 \end{bmatrix}</m>
        </p>
      </solution>
    </example>

    <p><nbsp/></p>

    <theorem xml:id="thm-transpose-properties" workspace="true">
      <title>Properties of Matrix Transpose</title>
      <statement>
        <ol>
          <li><m>(A^T)^T =</m> <m>A</m></li>
          <li><m>(A+B)^T =</m> <m>A^T + B^T</m></li>
          <li><m>(rA)^T =</m> <m>rA^T</m></li>
          <li><m>(AB)^T =</m> <m>B^TA^T</m></li>
        </ol>
      </statement>
    </theorem>

    <p><nbsp/></p>
  </page>

  <page xml:id="p-2-1-which-defined">
    <title>Example: Which Operations Are Defined?</title>

    <example xml:id="ex-which-operations-defined" workspace="true">
      <introduction>
        <p>Define</p>
        <me>
          A=
          \begin{bmatrix}
            1 \amp 0\\
            0 \amp 0
          \end{bmatrix},
          \qquad
          B=
          \begin{bmatrix}
            1 \amp 0 \amp 0\\
            0 \amp 0 \amp 8
          \end{bmatrix},
          \qquad
          C=
          \begin{bmatrix}
            1 \amp 0 \amp 0\\
            0 \amp 2 \amp 0\\
            0 \amp 0 \amp 2
          \end{bmatrix}.
        </me>

        <p>
          Which of these operations are defined, and what are the dimensions of the result?
        </p>
    </introduction>
        <task workspace="true">
          <statement><p><m>A + 3C</m></p></statement>
          <solution>
            <p>
                Note that <m>A </m> is a <m>2 \times 2</m> matrix while <m>3C</m> is a <m>3 \times 3</m> matrix. Therefore, the sum <m>A + 3C</m> is not defined.
            </p>
          </solution>
        </task>
        <task workspace="true">
          <statement><p><m>C(AB)^T</m></p></statement>
          <solution>
            <p>
                First, we can use Property (d) from <xref ref="thm-transpose-properties"/> to write <m>C(AB)^T = CB^TA^T</m>. Since <m>B </m> is a <m>2 \times 3</m> matrix, we have that <m>B^T </m> is a <m>3 \times 2</m> matrix. Since <m>A </m> is a <m>2 \times 2</m> matrix, we have that <m>A^T </m> is also a <m>2 \times 2</m> matrix. Thus, the product <m>CB^TA^T</m> is the product of a <m>3 \times 3</m> matrix with a <m>3 \times 2 </m> matrix with a <m>2 \times 2</m> matrix. Since all inner dimensions match, this product is defined.
            </p>
            <p>
                Let's calculate the product. One thing to note, even though matrix multiplication is not commutative, it is associative (see <xref ref="thm-properties-multiplication"/>), so we can either simplify the product by either computing <m>(CB^T)A</m> (mutliplying <m>C</m> and <m>B^T</m> first) or by computing <m>C(B^TA^T)</m> (multiplying <m>B^T</m> and <m>A^T</m> first). I choose whichever looks easier. It follows that <me>CB^TA^T = \begin{bmatrix} 1 \amp 0 \amp 0 \\ 0 \amp 2 \amp 0 \\ 0 \amp 0 \amp 2 \end{bmatrix}\begin{bmatrix} 1 \amp 0 \\ 0 \amp 0 \\ 0 \amp 8 \end{bmatrix}\begin{bmatrix}1 \amp 0 \\ 0 \amp 0 \end{bmatrix} = \begin{bmatrix} 1 \amp 0 \\ 0 \amp 0 \\ 0 \amp 16 \end{bmatrix}\begin{bmatrix} 1 \amp 0 \\ 0 \amp 0 \end{bmatrix} = \begin{bmatrix} 1 \amp 0 \\ 0 \amp 0 \\ 0 \amp 0 \end{bmatrix}</me>
            </p>
          </solution>
          </task>
        <task workspace="true">
            <statement><p><m>A + ABCB^T</m></p></statement>
            <solution>
                <p>
                    Note that <m>A </m> is a <m>2 \times 2</m> matrix, <m>B </m> is a <m>2 \times 3</m> matrix, <m>C </m> is a <m>3 \times 3</m> matrix, and <m>B^T</m> is a <m>3 \times 2</m> matrix. Therefore, all of the inner dimensions of the product <m>ABCB^T</m> match and results in a <m>2 \times 2</m> matrix. It follows that <m>A + ABCB^T</m> is defined.
                </p>
                <p>
                    We will simply this expression by making use of the associative property and simplifying <m>ABCB^T</m> by first multiplying <m>AB</m> and <m>CB^T</m>, then multiplying the resulting matrices. Note <m>\begin{eqnarray*} A + ABCB^T \amp = \amp \begin{bmatrix} 1 \amp 0 \\ 0 \amp 0 \end{bmatrix} + \left(\begin{bmatrix} 1 \amp 0 \\ 0 \amp 0 \end{bmatrix}\begin{bmatrix} 1 \amp 0 \amp 0 \\ 0 \amp 0 \amp 8 \end{bmatrix}\right) \left(\begin{bmatrix} 1 \amp 0 \amp 0 \\ 0 \amp 2 \amp 0 \\ 0 \amp 0 \amp 2 \end{bmatrix}\begin{bmatrix}1 \amp 0 \\ 0 \amp 0 \\ 0 \amp 8 \end{bmatrix}\right) \\ \amp = \amp \begin{bmatrix} 1 \amp 0 \\ 0 \amp 0 \end{bmatrix} + \begin{bmatrix} 1 \amp 0 \amp 0 \\ 0 \amp 0 \amp 0 \end{bmatrix}\begin{bmatrix}1 \amp 0 \\ 0 \amp 0 \\ 0 \amp 16 \end{bmatrix} \\ \amp = \amp \begin{bmatrix} 1 \amp 0 \\ 0 \amp 0 \end{bmatrix} + \begin{bmatrix} 1 \amp 0 \\ 0 \amp 0 \end{bmatrix} \\ \amp = \amp \begin{bmatrix} 2 \amp 0 \\ 0 \amp 0 \end{bmatrix}\end{eqnarray*}</m>
                </p>
            </solution>
        </task>
    </example>

    <p><nbsp/></p>
  </page>

  <page xml:id="p-2-1-matrix-powers">
    <title>Matrix Powers</title>

    <p>
      For any <m>n\times n</m> matrix and positive integer <m>k</m>,
      <m>A^k</m> is the product of <m>k</m> copies of <m>A</m>.
    </p>

    <me>A^k = AA\cdots A.</me>

    <example xml:id="ex-compute-a-power" workspace="true">
        <statement>
            <p>
                Compute <m>A^2</m> for <me>A = \begin{bmatrix} 3 \amp -2 \\ 5 \amp 1 \end{bmatrix}</me>
            </p>
        </statement>
        <solution>
            <p>
                <me>A^2 = \begin{bmatrix} 3 \amp -2 \\ 5 \amp 1 \end{bmatrix}\begin{bmatrix}3 \amp -2 \\ 5 \amp 1 \end{bmatrix} = \begin{bmatrix} -1 \amp -8 \\ 20 \amp -9 \end{bmatrix}</me>
            </p>
        </solution>
    </example>

    <p><nbsp/></p>

    <example xml:id="ex-compute-c-power" workspace="true">
      <statement>
        <p>Compute <m>B^8</m> for</p>
        <me>
          B=
          \begin{bmatrix}
            1 \amp 0 \amp 0\\
            0 \amp 2 \amp 0\\
            0 \amp 0 \amp 2
          \end{bmatrix}.
        </me>
      </statement>
      <solution>
        <p>
            As we saw in <xref ref="ex-compute-a-power"/>, you cannot distribute the exponent to the individual entries in the matrix. For <em>diagonal</em> matrices, you actually can. Note that <me>B^2 = \begin{bmatrix}1 \amp 0 \amp 0 \\ 0 \amp 2 \amp 0 \\ 0 \amp 0 \amp 2 \end{bmatrix}\begin{bmatrix}1 \amp 0 \amp 0 \\ 0 \amp 2 \amp 0 \\ 0 \amp 0 \amp 2 \end{bmatrix} = \begin{bmatrix} 1 \amp 0 \amp 0 \\ 0 \amp 4 \amp 0 \\ 0 \amp 0 \amp 4 \end{bmatrix} = \begin{bmatrix} 1^2 \amp 0 \amp 0 \\ 0 \amp 2^2 \amp 0 \\ 0 \amp 0 \amp 2^2 \end{bmatrix}</me>. Therefore, we have that <me>B^8 = \begin{bmatrix} 1^8 \amp 0 \amp 0 \\ 0 \amp 2^8 \amp 0 \\ 0 \amp 0 \amp 2^8 \end{bmatrix} = \begin{bmatrix} 1 \amp 0 \amp 0 \\ 0 \amp 256 \amp 0 \\ 0 \amp 0 \amp 256 \end{bmatrix}</me>. We will see an application of this to <em>diagonalizable</em> matrices in Section 5.3.
        </p>
      </solution>
    </example>

    <p><nbsp/></p>
  </page>


  


  <page xml:id="p-2-1-additional-examples">
    <title>Additional Examples</title>
    <example xml:id="ex-tf-identity-factorization">
        <introduction>
            <p>
                <em>True or False.</em> If false, explain briefly.
            </p>
        </introduction>
      <task workspace="true">
        <statement>
        <p>
          Let <m>n \in \mathbb{R}</m>. Then for any <m>n \times n</m> matrix <m></m>, we have <m>(I_n + A)(I_n - A) = I_n - A^2</m>.
        </p>
        </statement>
        <solution>
            <p>
                Recall from <xref ref="thm-properties-multiplication"/> that the Distributive Property applies to matrix mutliplication and addition. Therefore, we start with the distributive property to simply the product. <me>(I_n + A)(I_n - A) = I_nI_n + I_n(-A) + AI_n + A(-A)</me> By the multiplicative property of the identity matrix, we have that <m>I_nI_n = I_n</m> and <m>I_n(-A) = -A</m> and <m>AI_n = A</m>. Recall from our properties of matrix multipliation that we are allowed to commute scalars with matrix multiplication, just not matrices with matrix multiplication. Therefore, we can factor out the <m>-1</m> and rewrite <m>A(-A) = -AA = -A^2</m>. It follows that <me>(I_n + A)(I_n - A) = I_n - A + A - A^2 = I_n - A^2</me> since <m>-A + A</m> is the zero matrix, which doesn't change anything when you add it to a term. Therefore, we see that this statement is TRUE.
            </p>
        </solution>
        </task>
        <task workspace="true">
            <statement>
                <p>
                    Let <m>n \in \mathbb{R}</m>. For any <m>n \times n</m> matrices <m>A</m> and <m>B</m>, we have <m>(A+B)^2 = A^2 + B^2 + 2AB</m>.
                </p>
            </statement>
            <solution>
                <p>
                    Proceeding in a similar manner to the problem above, we see that <me>(A+B)^2 = (A+B)(A+B) = AA + AB + BA + BB</me>. We can rewrite <m>AA = A^2</m> and <m>BB = B^2</m>. Also, since matrix addition is commutative, we can move the terms <m>AB</m> and <m>BA</m> to the end. This leaves us with <me>(A+B)^2 = A^2 + B^2 + AB + BA</me>. Note that if <m>AB = BA</m>, then we could combine the middle terms into <m>2AB</m>. However, from the warning in <xref ref="thm-properties-multiplication"/>, we see that matrix multiplication is often not commutative. Therefore, we <em>cannot</em> replace <m>AB + BA</m> with <m>2AB</m>. This leads us to believe the statement is false.
                </p>
                <p>
                    We can prove it is false by giving a counterexample. Probably, pretty much anything we try will work since matrix commutation is very rare. Let 
                    <m>A = \begin{bmatrix} 1 \amp 2 \\ 3 \amp 4 \end{bmatrix}</m> and <m>B = \begin{bmatrix} 4 \amp 3 \\ 2 \amp 1 \end{bmatrix}</m>. Note that </p>
                    <p><m>\begin{eqnarray*}(A+B)^2   =  \left(\begin{bmatrix} 1 \amp 2 \\ 3 \amp 4 \end{bmatrix} + \begin{bmatrix} 4 \amp 3 \\ 2 \amp 1 \end{bmatrix}\right)^2   =  \begin{bmatrix} 5 \amp 5 \\ 5 \amp 5 \end{bmatrix}^2 \amp = \amp  \begin{bmatrix} 5 \amp 5 \\ 5 \amp 5 \end{bmatrix}\begin{bmatrix} 5 \amp 5 \\ 5 \amp 5 \end{bmatrix}\\ \amp = \amp \begin{bmatrix} 50 \amp 50 \\ 50 \amp 50 \end{bmatrix};\end{eqnarray*}</m></p>
                    <p> however, </p>
                <p><m>\begin{eqnarray*}A^2 + B^2 + 2AB \amp = \amp \begin{bmatrix} 1 \amp 2 \\ 3 \amp 4 \end{bmatrix}^2 + \begin{bmatrix} 4 \amp 3 \\ 2 \amp 1 \end{bmatrix}^2 + 2\begin{bmatrix}1 \amp 2 \\ 3\amp 4 \end{bmatrix}\begin{bmatrix} 4 \amp 3 \\ 2 \amp 1 \end{bmatrix}  \\ \amp = \amp \begin{bmatrix} 1 \amp 2 \\ 3 \amp 4 \end{bmatrix}\begin{bmatrix}1 \amp 2 \\ 3 \amp 4\end{bmatrix} + \begin{bmatrix} 4 \amp 3 \\ 2 \amp 1 \end{bmatrix}\begin{bmatrix} 4 \amp 3 \\ 2 \amp 1 \end{bmatrix} + 2\begin{bmatrix} 8 \amp 5 \\ 20 \amp 13 \end{bmatrix} \\ \amp = \amp \begin{bmatrix} 7 \amp 10 \\ 15 \amp 22 \end{bmatrix} + \begin{bmatrix} 22 \amp 15 \\ 10 \amp 7 \end{bmatrix} + \begin{bmatrix} 16 \amp 10 \\ 40 \amp 26 \end{bmatrix} \\ \amp = \amp \begin{bmatrix} 45 \amp 35 \\ 65 \amp 55 \end{bmatrix}\end{eqnarray*}</m></p>
                <p>Therefore, since <m>(A+B)^2 \neq A^2 + B^2 + 2AB</m> for these particular matrices, the statement must be FALSE.</p>
            </solution>
        </task>
    </example>
  </page>

</handout>